src/cbor/pulse/raw/CBOR.Pulse.Raw.Format.Match.fsti
@@ -26,6 +26,84 @@ val cbor_match_serialized_payload_tagged
   (r: raw_data_item)
 : Tot slprop
 
+val cbor_match_serialized_payload_array_share
+  (c: slice U8.t)
+  (p: perm)
+  (r: list raw_data_item)
+: stt_ghost unit emp_inames
+    (cbor_match_serialized_payload_array c p r)
+    (fun _ ->
+      cbor_match_serialized_payload_array c (p /. 2.0R) r **
+      cbor_match_serialized_payload_array c (p /. 2.0R) r
+    )
+
+val cbor_match_serialized_payload_array_gather
+  (c: slice U8.t)
+  (p1: perm)
+  (r1: list raw_data_item)
+  (p2: perm)
+  (r2: list raw_data_item)
+: stt_ghost unit emp_inames
+    (cbor_match_serialized_payload_array c p1 r1 **
+      cbor_match_serialized_payload_array c p2 r2
+    )
+    (fun _ ->
+      cbor_match_serialized_payload_array c (p1 +. p2) r1 **
+      pure (r1 == r2)
+    )
+
+val cbor_match_serialized_payload_map_share
+  (c: slice U8.t)
+  (p: perm)
+  (r: list (raw_data_item & raw_data_item))
+: stt_ghost unit emp_inames
+    (cbor_match_serialized_payload_map c p r)
+    (fun _ ->
+      cbor_match_serialized_payload_map c (p /. 2.0R) r **
+      cbor_match_serialized_payload_map c (p /. 2.0R) r
+    )
+
+val cbor_match_serialized_payload_map_gather
+  (c: slice U8.t)
+  (p1: perm)
+  (r1: list (raw_data_item & raw_data_item))
+  (p2: perm)
+  (r2: list (raw_data_item & raw_data_item))
+: stt_ghost unit emp_inames
+    (cbor_match_serialized_payload_map c p1 r1 **
+      cbor_match_serialized_payload_map c p2 r2
+    )
+    (fun _ ->
+      cbor_match_serialized_payload_map c (p1 +. p2) r1 **
+      pure (r1 == r2)
+    )
+
+val cbor_match_serialized_payload_tagged_share
+  (c: slice U8.t)
+  (p: perm)
+  (r: raw_data_item)
+: stt_ghost unit emp_inames
+    (cbor_match_serialized_payload_tagged c p r)
+    (fun _ ->
+      cbor_match_serialized_payload_tagged c (p /. 2.0R) r **
+      cbor_match_serialized_payload_tagged c (p /. 2.0R) r
+    )
+
+val cbor_match_serialized_payload_tagged_gather
+  (c: slice U8.t)
+  (p1: perm)
+  (r1: raw_data_item)
+  (p2: perm)
+  (r2: raw_data_item)
+: stt_ghost unit emp_inames
+    (cbor_match_serialized_payload_tagged c p1 r1 **
+      cbor_match_serialized_payload_tagged c p2 r2
+    )
+    (fun _ ->
+      cbor_match_serialized_payload_tagged c (p1 +. p2) r1 **
+      pure (r1 == r2)
+    )
+
 val cbor_match_serialized_payload_array_copy
   (c: slice U8.t)
   (p: perm)
